\documentclass{article}

\begin{document}

if i=j,
\[\frac{\partial{\frac{e^{a_{i}}}{\sum_{k=0}^{N}e^{a_{k}}}}}{\partial{a_{j}}}=\frac{\sum{{e^{a_{k}}}}.e^{a_{j}}-{e^{a_{i}}.e^{a_{j}}}}{{\sum{e^{a_{k}}}}^2}\]
\\
from hypothesis 1 $\bf{\sum_{k=0}^{N}{e^{a_{k}}}=e^{a_{j}}}$
\\
\[\frac{\partial{\frac{e^{a_{i}}}{\sum_{k=0}^{N}e^{a_{k}}}}}{\partial{a_{j}}}=\frac{e^{a_{j}}}{\sum{e^{a_{k}}}}.{\frac{\sum{e^{a_{k}}}-e^{a_{i}}}{\sum{e^{a_{k}}}}}\]
\\
\[\frac{\partial{\frac{e^{a_{i}}}{\sum_{k=0}^{N}e^{a_{k}}}}}{\partial{a_{j}}}={S_{j}}*(1-{S_{i}})\]
\\
\\
if i!=j,
from hypothesis 2 with condition i!=j
\\
\[\frac{\partial{\frac{e^{a_{i}}}{\sum_{k=0}^{N}e^{a_{k}}}}}{\partial{a_{j}}}=\frac{\sum{{e^{a_{k}}}}.0-{e^{a_{i}}.e^{a_{j}}}}{{\sum{e^{a_{k}}}}^2}\]
\\
\[\frac{\partial{\frac{e^{a_{i}}}{\sum_{k=0}^{N}e^{a_{k}}}}}{\partial{a_{j}}}=-{S_{j}}.{S_{i}}\]
\end{document}